---
title: "fisher_information_plackett_luce_three_runners"
output: html_document
date: "2022-08-14"
---

```{r setup, include=FALSE}
knitr::opts_chunk$set(echo = TRUE)
```

## Problem

We consider three runners, $a,b,c$ and a Plackett-Luce likelihood
function for the six possible orders.  We normalize so $a+b+c=1$ and
take $c=1-a-b$.

## $a\succ b\succ c$

prob = $\frac{ab}{1-a}$

$S=\log a+\log b-\log(1-a)$

$\partial S/\partial a = a^{-1} + (1-a)^{-1}$

$\partial S/\partial b=b^{-1}$

$\partial^2 S/\partial a^2=-a^{-2} +(1-a)^{-2}$

$\partial^2 S/\partial b^2 = -b^{-2}$

$\partial^2 S/\partial a\partial b=0$ 

## $a\succ c\succ b$

prob = $\frac{a(1-a-b)}{1-a}$

$S=\log a-\log(1-a) +\log(1-a-b)$

$\partial S/\partial a = a^{-1} + (1-a)^{-1} + (1-a-b)^{-1}$

$\partial S/\partial b = (1-a-b)^{-1}$

$\partial ^2S/\partial a^2 = -a^{-2}+(1-a)^{-2} + (1-a-b)^{-2}$

$\partial^2S/\partial a\partial b = (1-a-b)^{-2}$

## $b\succ a\succ c$

prob = $\frac{ba}{1-b}$

$S=\log a +\log b-\log(1-b)$

$\partial S/\partial a = a^{-1}$

$\partial S/\partial b = b^{-1} +(1-b)^{-1}$

$\partial^2S/\partial a^2 = -a^{-2}$

$\partial^2S/\partial b^2=-b^{-2} +(1-b)^{-2}$

$\partial^2S/\partial a\partial b=0$

## $b\succ c\succ a$

prob = $\frac{a(1-a-b)}{1-b}$

$S=\log a + \log(1-a-b) - \log(1-b)$

$\partial S/\partial a=a^{-1} -(1-a-b)^{-1}$

$\partial S/\partial b=-(1-a-b)^{-1} - (1-b)^{-1}$

$\partial^2S\partial a^2=-a^{-2} -(1-a-b)^{-2}$

$\partial^2S/\partial b^2 =-(1-a-b)^{-2} -(1-b)^{-2}$

$\partial^2S/\partial a\partial b=-(1-a-b)^{-2}$

## $c\succ a\succ b$

prob=$\frac{a(1-a-b)}{a+b}$

$S=\log a + \log(1-a-b) -\log(a+b)$

$\partial S/\partial a=a^{-1} -(1-a-b)^{-1} -(a+b)^{-1}$

$\partial S/\partial  b=-(1-a-b)^{-1}-(a+b)^{-1}$

$\partial^2S/\partial a^2=-a^{-2} -(1-a-b)^{-2} +(a+b)^{-2}$

$\partial^2S/\partial b^2=-(1-a-b)^{-2} +(a+b)^{-2}$

$\partial^2S/\partial a\partial b=-(1-a-b)^{-2}+(a+b)^{-2}$

## $c\succ b\succ a$

prob=$\frac{b(1-a-b)}{1-b}$

$S=\log b+\log(1-a-b) -\log(1-b)$

$\partial S/\partial a=-(1-a-b)^{-1}$

$\partial S/\partial b=b^{-1}+(1-b)^{-1} -(1-a-b)^{-1}$

$\partial^2S/\partial a^2=-(1-a-b)^{-2}$

$\partial^2S/\partial b^2=-b^{-2} +(1-b)^{-2}-(1-a-b)^{-2}$

$\partial^2S/\partial a\partial b=-(1-a-b)^{-2}$




